tests/fstar/misc/Loops.Clauses.fst
@@ -5,6 +5,10 @@ open Loops.Types
 
 #set-options "--z3rlimit 50 --fuel 1 --ifuel 1"
 
+(** [loops::sum]: decreases clause *)
+unfold let sum_decreases (max : u32) (i : u32) (s : u32) : nat =
+  if i <= max then max - i else 0
+
 (** [loops::list_nth_mut_loop]: decreases clause *)
 unfold
 let list_nth_mut_loop_decreases (t : Type0) (ls : list_t t) (i : u32) : nat =
